<section>
  <title>The Squeeze Theorem</title>
  <subsection>
    <title>Learning Goals</title>
    <ul>
      <li>
        <p>
          Learn the Squeeze Theorem and how its statement is interpreted visually in terms of the graphs of functions.
        </p>
      </li>
      <li>
        <p>
          Use a few known inequalities involving sine, cosine,
          and arctangent in order to apply the Squeeze Theorem to calculate limits.
        </p>
      </li>
      <li>
        <p>
          See how to use the Squeeze Theorem to rigorously prove that the derivative of sine is cosine and recognize the importance of avoiding circular logic in mathematical deduction.
        </p>
      </li>
    </ul>
  </subsection>
  <subsection>
    <title>Statement of the Squeeze Theorem</title>
    <p>
      Another useful tool for calculating new types of limits is the Squeeze Theorem.
      This theorem says that if the output of a function <m>f(x)</m> is always bounded between a "lower function" <m>l(x)</m> and an "upper function" <m>u(x)</m>,
      and if the lower and upper functions approach the same value <m>L</m> as <m>x\to c</m>,
      then <m>f(x)</m> gets squeezed between the lower and upper functions and also approaches <m>L</m> as <m>x\to c</m>
    </p>
    <theorem>
      <title>The Squeeze Theorem for Limits</title>
      <statement>
        <p>
          If <m>l(x)\leq f(x)\leq u(x)</m> for all <m>x</m> near <m>c</m>,
          not not necessarily at <m>x=c</m>,
          and if <m>\ds\lim_{x\to c}l(x)</m> and
          <m>\ds\lim_{x\to c} u(x)</m> are both equal to <m>L</m>,
          then <m>\ds\lim_{x\to c}f(x) = L</m>.
        </p>
        <p>
          <image width="51%" source="SqueezeTheoremPic.png"/>
        </p>
        <p>
          The theorem holds for <m>x\to\pm\infty</m> and <m>x\to c^\pm</m>.
        </p>
      </statement>
    </theorem>
    <remark>
      <p>
        The Squeeze Theorem is also called the Sandwich Theorem.
        You can think of the lower and upper functions as pieces of bread that make a sandwich with the middle function <m>f(x)</m>.
      </p>
    </remark>
    <example xml:id="ex_SqueezeTheorem2">
      <statement>
        <p>
          For example,
          the figure that follows shows a function <m>f</m> that is sandwiched between two functions <m>u</m> and <m>l</m> as <m>x\to 0</m>.
          Since <m>u(x)</m> and <m>l(x)</m> have the same limit as <m>x\to 0</m> and <m>f(x)</m> is squeezed between them,
          we know that <m>f(x)</m> must share that same limit as <m>x\to 0</m>.
        </p>
        <p>
          <image width="46%" source="TaalmanPage152.png"/>
        </p>
      </statement>
    </example>
    <p>
      The Squeeze Theorem gives us a way to compute limits algebraically that we may suspect to be true based on the graph of a function,
      as demonstrated in the next example.
    </p>
    <example>
      <statement>
        <p>
          Consider the graph of the function <m>f(x) = x^2\sin\frac{1}{x}</m> shown below:
        </p>
        <p>
          <image width="46%" source="TaalmanPage153a.png"/>
        </p>
        <p>
          From this graph it seems reasonable that <m>\ds\lim_{x\to0}x^2\sin \frac{1}{x} = 0</m>.
          We can use the Squeeze Theorem to find this limit algebraically.
          The sine function has outputs that are always between <m>-1</m> and <m>1</m>,
          regardless of the input.
          Therefore,
          <me>
            -1\leq \sin\frac{1}{x}\leq 1
          </me>
          where we are substituting <m>\theta = \frac{1}{x}</m> in the inequality <m>-1\leq \sin \theta\leq 1</m>.
          Multiplying both sides of the above inequality by <m>x^2</m>,
          <me>
            -x^2\leq x^2\sin\frac{1}{x}\leq x^2
          </me>.
        </p>
        <p>
          Note that we do not have to worry about flipping the order of the inequalities because <m>x^2\geq 0</m>,
          so we know we are not multiplying by a negative number.
          We can see this relationship between the graphs of <m>x^2\sin\frac{1}{x}</m>,
          <m>-x^2</m>,
          and <m>x^2</m> in the graph below:
        </p>
        <p>
          <image width="46%" source="TaalmanPage153a.png"/>
        </p>
        <p>
          We know that <m>\ds\lim_{x\to 0} -x^2 = 0</m> and <m>\ds\lim_{x\to 0}x^2 = 0</m>.
          Therefore by the Squeeze Theorem we must also have <m>\ds\lim_{x\to 0}x^2\sin\frac{1}{x} = 0</m>.
        </p>
      </statement>
    </example>
    <exercise>
      <statement>
        <p>
          In <xref ref="ex_SqueezeTheorem2">Example</xref>,
          why was it important that <m>x^2</m> is not negative?
        </p>
      </statement>
    </exercise>
    <remark>
      <p>
        There are three important hypotheses that must be satisfied in order to use the Squeeze Theorem:
        <ul>
          <li>
            <p>
              We must have the inequality
              <m>l(x)\leq f(x)\leq u(x)</m> for <m>x</m> near <m>c</m>.
            </p>
          </li>
          <li>
            <p>
              The limits <m>\ds\lim_{x\to c} l(x)</m> and <m>\ds\lim_{x\to c}u(x)</m> must exist
              (and be finite).
            </p>
          </li>
          <li>
            <p>
              The limits <m>\ds\lim_{x\to c} l(x)</m> and
              <m>\ds\lim_{x\to c}u(x)</m> must be equal to each other.
            </p>
          </li>
        </ul>
      </p>
      <p>
        Once those hypotheses are satisfied,
        the conclusion of the theorem is that
        <m>\ds\lim_{x\to c} f(x)</m> is the same as the limits
        <m>\ds\lim_{x\to c} l(x)</m> and <m>\ds\lim_{x\to c}u(x)</m>.
      </p>
    </remark>
    <exercise>
      <statement>
        <p>
          Use
          <url href="https://www.desmos.com/calculator">Desmos</url>
          to graph <m>f(x) = x^2\ln(|x|)</m>,
          <m>g(x)=|x|</m>, and <m>h(x) = -|x|</m>.
          <ol marker="labelalphitemsep5pttopsep10pt">
            <li>
              <p>
                Verify that for <m>x</m> near <m>0</m>,
                <m>-|x|\leq x^2\ln|x|\leq |x|</m>.
                How close to <m>x=0</m> do we need to be in order for this inequality to be true?
              </p>
            </li>
            <li>
              <p>
                Calculate <m>\ds\lim_{x\to 0}-|x|</m> and <m>\ds\lim_{x\to 0}|x|</m>.
                What are they both equal to?
              </p>
            </li>
            <li>
              <p>
                Fill in the blanks: "By the Squeeze Theorem,
                we can conclude that <m>\lim_{x\to\rule[-.25em]{.2in}{.5pt}}x^2\ln|x| = \rule[-.25em]{.5in}{.5pt}</m>."
              </p>
            </li>
          </ol>
        </p>
      </statement>
    </exercise>
  </subsection>
  <subsection>
    <title>Using the Squeeze Theorem</title>
    <p>
      In general, finding the inequality <m>l(x)\leq f(x)\leq u(x)</m> is very difficult.
      However, there are three inequalities that are particularly useful as a starting point for applying the Squeeze Theorem:
      <me>
        -1\leq \sin\theta\leq 1
      </me>
      <me>
        -1\leq \cos\theta\leq 1
      </me>
      <me>
        -\frac{\pi}{2}\lt \arctan\theta\lt \frac{\pi}{2}
      </me>
    </p>
    <p>
      For limits involving sine, cosine, or arctangent,
      we can use these inequalities as a starting point for building up to an inequality involving the function we wish to know the limit of.
    </p>
    <example>
      <statement>
        <p>
          Use the Squeeze Theorem to find any horizontal asymptotes of <m>f(x) = \frac{\sin x}{x}</m>.
        </p>
      </statement>
      <solution>
        <p>
          We wish to determine <m>\ds\lim_{x\to\infty} \frac{\sin x}{x}</m> and <m>\ds\lim_{x\to-\infty} \frac{\sin x}{x}</m>.
          Starting with <m>x\to\infty</m>,
          we begin with the inequality
          <me>
            -1\leq \sin x\leq 1
          </me>.
        </p>
        <p>
          We are interested in the function <m>\frac{\sin x}{x}</m>,
          so we can divide by <m>x</m> in order to have the middle function equal to <m>\frac{\sin x}{x}</m>;
          this is what we want in order to apply the Squeeze Theorem.
          As <m>x\to\infty</m>,
          we know that <m>x>0</m> and so dividing by <m>x</m> does not flip the inequality:
          <me>
            -\frac{1}{x}\leq \frac{\sin x}{x}\leq\frac{1}{x}
          </me>.
          If we take the limit of the bounding functions,
          they are both equal to zero:
          <me>
            \lim_{x\to\infty}-\frac{1}{x} = 0\text{ and } \lim_{x\to\infty}\frac{1}{x} = 0
          </me>
        </p>
        <p>
          Hence by the Squeeze Theorem,
          the limit of the middle function <m>\frac{\sin x}{x}</m> is the same:
          <me>
            \lim_{x\to\infty}\frac{\sin x}{x} = 0
          </me>
        </p>
        <p>
          Let's now consider <m>x\to-\infty</m>.
          We can still start with
          <me>
            -1\leq \sin x\leq 1
          </me>
          but now <m>x\lt 0</m> so when we divide by <m>x</m>,
          we must flip the inequalities:
          <me>
            -\frac{1}{x}\geq \frac{\sin x}{x}\geq\frac{1}{x}
          </me>.
          We still have that the limits of both bounding function are equal to zero:
          <me>
            \lim_{x\to-\infty}-\frac{1}{x} = 0\text{ and } \lim_{x\to-\infty}\frac{1}{x} = 0
          </me>
          so by the Squeeze Theorem,
          the limit of the middle function <m>\frac{\sin x}{x}</m> is the same:
          <me>
            \lim_{x\to-\infty}\frac{\sin x}{x} = 0
          </me>
        </p>
        <p>
          Thus overall, the function
          <m>f(x) = \frac{\sin x}{x}</m> has left and right horizontal asymptotes at <m>y=0</m>.
        </p>
      </solution>
    </example>
    <exercise xml:id="ex_squeezesinxoverx">
      <statement>
        <p>
          Explain why we <em>cannot</em> use the Squeeze Theorem and the inequality
          <me>
            -\frac{1}{x}\leq \frac{\sin x}{x}\leq\frac{1}{x}
          </me>
          to determine <m>\ds\lim_{x\to 0}\frac{\sin x}{x}</m>.
        </p>
      </statement>
    </exercise>
    <example>
      <statement>
        <p>
          Use the Squeeze Theorem to calculate
          <me>
            \lim_{x\to\infty}\frac{3x^2+\cos x^2}{x^2+1}
          </me>
        </p>
      </statement>
      <solution>
        <p>
          Beginning with the inequality
          <me>
            -1\leq \cos \theta\leq 1
          </me>,
          we build up the middle of the inequality until it is equal to the given function:
          <m>\frac{3x^2+\cos x^2}{x^2+1}</m>.
        </p>
        <p>
          To start, we use <m>\theta = x^2</m> and have
          <me>
            -1\leq \cos x^2\leq 1
          </me>
        </p>
        <p>
          Next, add <m>3x^2</m> to both sides of the inequality:
          <me>
            3x^2-1\leq 3x^2+\cos x^2\leq 3x^2+1
          </me>
        </p>
        <p>
          Lastly, divide all three parts by <m>x^2+1</m>.
          Note that the expression <m>x^2+1</m> is positive for all values of <m>x</m>,
          so we do not have to worry about flipping the inequality:
          <me>
            \frac{3x^2-1}{x^2+1}\leq \frac{3x^2+\cos x^2}{x^2+1}\leq \frac{3x^2+1}{x^2+1}
          </me>
        </p>
        <p>
          Now from our previous work with rational functions, we know that
          <me>
            \lim_{x\to\infty}\frac{3x^2-1}{x^2+1} =3 \text{ and }  \lim_{x\to\infty}\frac{3x^2+1}{x^2+1}=3
          </me>
        </p>
        <p>
          Hence by the Squeeze Theorem,
          <me>
            \lim_{x\to\infty}\frac{3x^2+\cos x^2}{x^2+1}=3
          </me>
        </p>
      </solution>
    </example>
    <exercise>
      <statement>
        <p>
          Start with the inequality <m>-\frac{\pi}{2}\lt \arctan\theta\lt \frac{\pi}{2}</m>.
          What steps do you need to follow in order to conclude that
          <me>
            \left(5-\frac{\pi}{2x^4}\right)\lt  \left(5+\frac{\arctan(\pi x)}{x^4}\right)\lt \left(5+\frac{\pi}{2x^4}\right)?
          </me>
        </p>
        <p>
          Use this inequality and the Squeeze Theorem to calculate <m>\ds\lim_{x\to \infty} \left(5+\frac{\arctan(\pi x)}{x^4}\right)</m>
        </p>
      </statement>
    </exercise>
  </subsection>
  <subsection>
    <title>The Derivatives of Sine and Cosine: Rigorous Proofs</title>
    <p>
      In <xref ref="sec_derivativesoftrigfunctions">Section</xref>,
      we inferred that the derivative of the sine function is the cosine function by observing the behavior of the associated slope function of sine,
      and likewise that the derivative of the cosine function is the negative of the sine function.
      However, that is not a mathematically rigorous proof.
      In this section, we formally prove what you already know:
      <me>
        \frac{d}{dx}(\sin x) = \cos x\text{ and } \frac{d}{dx}(\cos x) = -\sin x
      </me>.
      There is a very complicated application of the Squeeze Theorem necessary for this proof,
      which is why we include it here.
      However, it is much harder than anything we will ask you to do.
      It is worth reading through this section to see how all of the different ideas we've developed fit together,
      but don't feel like you have to follow every single detail.
      In particular,
      the two special limits calculated via the Squeeze Theorem will be found using different methods in the next section.
    </p>
    <p>
      In order to calculate the derivative of <m>\sin x</m>,
      we start with the limit definition of the derivative:
      <me>
        \begin{aligned}\frac{d}{dx}(\sin x) \amp = \lim_{h\to 0}\frac{\sin (x+h)-\sin x}{h} \amp  \leftarrow\text{ definition of the derivative } \\ \amp = \lim_{h\to 0}\frac{(\sin x\cos h+\sin h\cos x)-\sin x}{h}\amp  \leftarrow\text{ sum identity for sine } \\ \amp = \lim_{h\to 0}\frac{\sin x(\cos h-1)+\sin h\cos x}{h}\amp  \leftarrow\text{ rearrange and factor } \\ \amp = \lim_{h\to 0}\left(\sin x\frac{\cos h-1}{h}+\cos x\frac{\sin h}{h}\right)\amp  \leftarrow\text{ factor more } \\ \amp =\sin x\left(\lim_{h\to 0}\frac{\cos h-1}{h}\right)+\cos x\left(\lim_{h\to 0}\frac{\sin h}{h}\right)\amp  \leftarrow\text{ use limit rules and factor again } \end{aligned}
      </me>
    </p>
    <p>
      In the last step above,
      notice that since the variable in the limit is <m>h</m>,
      not <m>x</m>,
      we can factor the <m>\sin x</m> and <m>\cos x</m> out of the limits as "constants."
    </p>
    <p>
      We now need to calculate the limits
      <m>\ds\lim_{h\to 0}\frac{\cos h-1}{h}</m> and <m>\ds\lim_{h\to 0}\frac{\sin h}{h}</m>,
      which both have the form <m>\frac{0}{0}</m>.
      However, we cannot use L'H&#xf4;pital's rule!
      Why??? <em>This is a very important piece of logic:
      we are trying to prove the formula for the derivative of the sine function,
      so we cannot use the derivative of the sine function while proving it.</em>
      That would be what is called "circular logic:" when we rely on the thing we are trying to prove in order to prove it.
    </p>
    <exercise>
      <statement>
        <p>
          Give an example from your own experience that demonstrates circular logic,
          meaning an argument that uses a "fact" in order to justify that same "fact."
        </p>
      </statement>
    </exercise>
    <p>
      In order to evaluate <m>\ds\lim_{h\to 0}\frac{\sin h}{h}</m>,
      we use the Squeeze Theorem.
      However, as observed in <xref ref="ex_squeezesinxoverx">Exercise</xref>,
      we cannot use the inequality <m>-\frac{1}{h}\leq \frac{\sin h}{h}\leq \frac{1}{h}</m> for this limit.
      (In that exercise, you were asked to explain why.)
    </p>
    <p>
      Instead, consider the picture below that shows a triangle appropriate for small,
      positive values of <m>\theta</m>
      (so values close to <m>0^+</m>).
    </p>
    <p>
      <image width="37%" source="TaalmanPage427a.png"/>
    </p>
    <p>
      In the smaller triangle,
      the hypotenuse is 1, the height of the side opposite <m>\theta</m> is <m>\sin\theta</m>,
      and the length of the adjacent side is <m>\cos\theta</m>.
      In the larger triangle, the adjacent side has length 1.
      We can find the height of the opposite side using similar triangles:
      <me>
        \frac{\text{ opp } }{\text{ adj } } = \frac{\sin\theta}{\cos\theta} = \frac{\text{?} }{1}
      </me>
      and so the height of the unknown opposite side of the larger triangle must be <m>\frac{\sin\theta}{\cos\theta} = \tan\theta</m>.
      Lastly, the length of the arc from the bottom right corner of the larger triangle to the top right corner of the smaller triangle has length <m>\theta</m> because the hypotenuse of the smaller triangle is <m>1</m>;
      radians are specifically defined to be equal to the arc length around the circle of radius 1.
      Comparing these three lengths,
      we see that <m>\sin\theta</m> is the smallest,
      <m>\tan\theta</m> is the largest,
      and <m>\theta</m> is between these two.
      Hence we have the inequality
      <me>
        \sin\theta\leq \theta\leq \tan\theta
      </me>.
      Dividing through by <m>\sin\theta</m>,
      which is positive as long as <m>\theta\to0^+</m>,
      and remembering that <m>\tan\theta = \frac{\sin\theta}{\cos\theta}</m>,
      <me>
        1\leq \frac{\theta}{\sin\theta}\leq \frac{1}{\cos\theta}
      </me>.
      Since all of the expressions in this chain of inequalities are positive,
      we can take reciprocals and flip the inequalities to obtain:
      <me>
        1\geq \frac{\sin\theta}{\theta}\geq \cos\theta
      </me>.
      We justified this inequality for
      <m>\theta\to0^+</m> but it is also true for <m>\theta\to0^-</m>,
      only we must draw the picture in the fourth quadrant and the arithmetic has a few more flippings of inequalities since the quantities involved are negative.
    </p>
    <p>
      Now by applying the Squeeze Theorem to this inequality,
      we have <m>\ds\lim_{\theta\to 0}1 =\ds\lim_{\theta\to0}\cos\theta = 1</m>, hence
      <me>
        \lim_{\theta\to 0}\frac{\sin\theta}{\theta} = 1
      </me>.
    </p>
    <p>
      In particular, <m>\ds\lim_{h\to0}\frac{\sin h}{h} = 1</m>.
      We also needed to compute <m>\ds\lim_{h\to 0}\frac{\cos h-1}{h}</m>.
      In order to do this, we let
      <m>h=2\theta</m> and use the double-angle identity <m>\cos2\theta = 1-\sin^2\theta</m>:
      <me>
        \begin{aligned}\lim_{h\to 0}\frac{1-\cos h}{h} \amp = \lim_{\theta\to 0}\frac{1-\cos2\theta}{2\theta}\amp \leftarrow\text{ let } h=2\theta\\ \amp = \lim_{\theta\to 0} \frac{1-(1-2\sin^2\theta)}{2\theta}\amp \leftarrow\text{ use } \cos2\theta = 1-\sin^2\theta\\ \amp =\lim_{\theta\to 0}\frac{\sin^2\theta}{\theta}\amp \leftarrow\text{ simplify } \\ \amp =\lim_{\theta\to 0}\theta\cdot\frac{(\sin\theta)^2}{\theta^2}\amp \leftarrow\text{ multiply and divide by an extra } \theta\\ \amp =\left(\lim_{\theta\to 0}\theta\right)\cdot\left(\lim_{\theta\to 0}\frac{\sin\theta}{\theta}\right)^2\amp \leftarrow\text{ limit rules } \\ \amp = (0)(1)^2\amp \leftarrow\text{ use that } \lim_{\theta\to0}\frac{\sin\theta}{\theta}=1\\ \amp = 0 \amp \leftarrow\text{ Voila! } \end{aligned}
      </me>
    </p>
    <p>
      Thus we see that
      <me>
        \lim_{h\to 0}\frac{1-\cos h}{h}  = \lim_{h\to 0}-\frac{\cos h-1}{h} = 0
      </me>
      and returning to our calculation of the derivative:
      <me>
        \begin{aligned}\frac{d}{dx}(\sin x) \amp =\sin x\left(\lim_{h\to 0}\frac{\cos h-1}{h}\right)+\cos x\left(\lim_{h\to 0}\frac{\sin h}{h}\right)\amp  \leftarrow\text{ where we left off before } \\ \amp = \sin x(0)+\cos x(1)\amp \leftarrow\text{ using the limits we calculated } \\ \amp = \cos x\amp \leftarrow\text{ simplifying } \end{aligned}
      </me>
    </p>
    <p>
      We can use the sum identity for cosine and the same two limits in order to calculate the derivative of cosine using the limit definition of the derivative:
      <me>
        \begin{aligned}\frac{d}{dx}(\cos x) \amp = \lim_{h\to 0}\frac{\cos (x+h)-\cos x}{h} \amp  \leftarrow\text{ definition of the derivative } \\ \amp = \lim_{h\to 0}\frac{(\cos x\cos h-\sin x\sin h)-\cos x}{h}\amp  \leftarrow\text{ sum identity for cosine } \\ \amp = \lim_{h\to 0}\frac{\cos x(\cos h-1)-\sin x\sin h}{h}\amp  \leftarrow\text{ rearrange and factor } \\ \amp = \lim_{h\to 0}\left(\cos x\frac{\cos h-1}{h}-\sin x\frac{\sin h}{h}\right)\amp  \leftarrow\text{ factor more } \\ \amp =\cos x\left(\lim_{h\to 0}\frac{\cos h-1}{h}\right)-\sin x\left(\lim_{h\to 0}\frac{\sin h}{h}\right)\amp  \leftarrow\text{ use limit rules and factor again } \\ \amp = \cos x(0)-\sin x(1)\amp \leftarrow\text{ using the limits we calculated } \\ \amp = -\sin x\amp \leftarrow\text{ simplifying } \end{aligned}
      </me>
    </p>
  </subsection>
  <subsection>
    <title>Summary</title>
    <p>
      The following terms and theorems were introduced in this section:
    </p>
    The Squeeze Theorem; circular logic
    <p>
      <em>Key ideas:</em> When a function is bounded above and below at a point by functions that approach a particular limit,
      then the bounded function approaches that same limit.
      We can use the ranges of the sine, cosine,
      and arctangent functions to our advantage in coming up with an inequality with which to apply the Squeeze Theorem.
      Other than being able to start with one of these three inequalities,
      it is very hard to find an inequality to use for the Squeeze Theorem.
    </p>
    <p>
      <em>Other ideas reinforced:</em>
      Mathematical Theorems must be proven rigorously with deductive arguments that use known axioms and facts,
      avoiding circular logic
      (meaning assuming what you wish to know in order to prove that it is true).
      This is sometimes incredibly difficult and tedious.
    </p>
    <p>
      \fbox{\fbox{ End of Section 8.2}}
    </p>
    <p>
      \rule{1.1\textwidth}{2pt}
    </p>
  </subsection>
</section>