<section>
  <title>Composition of Functions</title>
  <introduction>
    <p>
          <idx><h>Functions</h><h>Composition of Functions</h></idx>
    </p>
  </introduction>
  <subsection>
    <title>Learning Goals</title>
    <ul>
      <li>
        <p>
          Understand what it means to compose two functions
        </p>
      </li>
      <li>
        <p>
          Calculate values of compositions of functions given tables, graphs,
          or formulas
        </p>
      </li>
      <li>
        <p>
          Simplify the formula for a composition of functions
        </p>
      </li>
      <li>
        <p>
          Determine the domain of a composition of functions
        </p>
      </li>
      <li>
        <p>
          See an example where composition of functions is vital to studying calculus
        </p>
      </li>
    </ul>
  </subsection>
  <subsection>
    <title>Motivation and Examples</title>
    <p>
      Recall that a function, by definition,
      is a process that takes a collection of inputs and produces a corresponding collection of outputs in such a way that the process produces one and only one output value for any single input value.
      Because every function is a process,
      it makes sense to think that it may be possible to take two function processes and do one of the processes first,
      and then apply the second process to the result.
    </p>
    <p>
      Recall Dolbear's function, <m>F=D(N)=40+0.25N</m>,
      from Example <xref ref="ex_DolbearTake1" autoname="yes"/> that relates the number <m>N</m> of chirps per minute from a snowy cricket to the Fahrenheit temperature,
      <m>F</m>.
    </p>
    <p>
      The Celsius and Fahrenheit temperature scales are connected by a linear function.
      Indeed, the function that converts Fahrenheit to Celsius is
      <me>
        C = G(F) = \frac{5}{9}(F-32)
      </me>
    </p>
    <p>
      For instance,
      a Fahrenheit temperature of 32 degrees corresponds to <m>C=G(32) = 0</m> degrees Celsius.
    </p>
    <p>
      If we are given a number of chirps, <m>N</m>,
      we can combine the two processes given by Dolbear's function and the conversion from Fahrenheit to Celsius to obtain a new function <m>C=H(N)</m> that takes as input the number of chirps per minute and gives as output the temperature in degrees Celsius.
    </p>
    <example>
      <statement>
        <p>
          Suppose that we observe 80 chirps per minute.
          What is the temperature in degrees Celsius?
        </p>
        <p>
          First, we compute that the temperature in degrees Fahrenheit is
          <me>
            F = D(80) = 40+0.25(80) = 60
          </me>.
        </p>
        <p>
          Then, we compute that the temperature in degrees Celsius is
          <me>
            C = G(60) = \frac{5}{9}(60-32) = \frac{140}{9} =15\frac{5}{9}^\circ C
          </me>
        </p>
      </statement>
    </example>
    <p>
      We could do this individually for each value of <m>N</m>,
      but it would be more convenient to have a single formula that can go directly from number of chirps per minute to degrees Celsius.
      In the above example,
      we took the output <m>F=D(80)</m> and used it as the input for the temperature conversion <m>C=G(F)</m> from Fahrenheit to Celsius.
      We can do the same thing using the variable <m>N</m> instead of the explicit input <m>N=80</m>:
    </p>
    <example>
      <statement>
        <p>
          Determine a formula for the new function <m>C=H(N)</m> that takes as input the number <m>N</m> of cricket chirps per minute and gives as output the temperature <m>C</m> in degrees Celsius.
        </p>
        <p>
          Using <m>F=D(N)</m> as the input for the function <m>C=G(F)</m>,
          we simplify to find a formula directly from <m>N</m> to <m>C</m> that does not involve the variable <m>F</m>:
          <me>
            \begin{aligned}C \amp = G(F)\\ \amp = G(D(N))\\ \amp = \frac{5}{9}(D(N)-32)\\ \amp = \frac{5}{9}((40+0.25N)-32)\\ \amp =\frac{5}{9}(8+0.25N) \end{aligned}
          </me>
        </p>
        <p>
          So the function <m>C=H(N)</m> is given by
          <me>
            C = \frac{5}{9}(8+0.25N)
          </me>
        </p>
      </statement>
    </example>
    <p>
      There is, of course,
      a shorthand notation for this process of using the output of <m>D</m> as the input of <m>G</m>:
      <me>
        H=G\circ D
      </me>
    </p>
    <p>
      <m>G\circ D</m> is the function that first applies the process given by the function <m>D</m> and then applies the process given by the function <m>G</m>.
      Two natural questions we could begin by asking are:
    </p>
    "What is the domain of <m>H = G\circ D</m>?" <nbsp/><nbsp/> and <nbsp/><nbsp/> "What is the range of <m>H=G\circ D</m>?"
    <example>
      <statement>
        <p>
          Find the domain and range of the function <m>C=H(N)</m>.
        </p>
        <p>
          We established in Example <xref ref="ex_DolbearTake2" autoname="yes"/> that <m>F=D(N)</m> has a domain of
          <m>[40,180]</m> cricket chirps per minute and a corresponding range of <m>[50,85]</m> degrees Fahrenheit.
        </p>
        <p>
          The domain for <m>H=G\circ D</m> is the inputs of <m>H</m>,
          so is also the inputs of <m>D</m> as that is the function that is applied first.
          Thus we can use the same set of <m>N</m>-values and the domain of <m>H</m> is also <m>[40,180]</m>.
        </p>
        <p>
          In order to determine the range,
          we must find the resulting degrees Celsius from the range of degrees Fahrenheit of <m>[50,85]</m>.
          <me>
            G(50) = \frac{5}{9}(50-32) = 10
          </me>
          and
          <me>
            G(85) = \frac{5}{9}(85-32) = \frac{265}{9}= 29\frac{4}{9}
          </me>.
          We know that a linear function's range will stay within these two values based on the shape of the graph.
          Thus the range of <m>H</m> is in degrees Celsius instead of Fahrenheit,
          and is <m>[10,29\frac{4}{9}]</m>.
        </p>
      </statement>
    </example>
  </subsection>
  <subsection>
    <title>Definition of Composition of Functions</title>
    <p>
      Suppose we have two function, <m>g</m> and <m>f</m>.
      <m>g</m> has domain <m>A</m> and range <m>B</m>,
      while <m>f</m> has domain <m>B</m> and range <m>C</m>.
      We write <m>g</m> and <m>f</m> along with their domains and ranges as <m>g:A\to B</m> and <m>f:B\to C</m>.
      As long as the range of <m>g</m> matches the domain of <m>f</m>,
      it is possible to link the two processes together to create a new process that we call the
      <em>composition of <m>f</m> and <m>g</m></em>.
    </p>
    <definition>
      <title>The Composition of Two Functions</title>
      <statement>
        <p>
          If <m>f</m> and <m>g</m> are functions such that <m>g:A\to B</m> and <m>f:B\to C</m>,
          we define the <em>composition of <m>f</m> and <m>g</m></em>
          to be the new function <m>h:A\to C</m> given by
          <me>
            h(t) = f(g(x))
          </me>.
          We also sometimes use the notation <m>h = f\circ g</m>,
          where <m>f\circ g</m> is the single function defined by
          <me>
            (f\circ g)(x) = f(g(x))
          </me>
        </p>
      </statement>
    </definition>
    <figure xml:id="fig_comositionoffunctions">
      <caption>The composition <m>(f\circ g)(x) = f(g(x))</m> uses the outputs <m>g(x)</m> as the inputs of <m>f</m>.</caption>
      <image width="93%" source="CompositionOfFunctions.png"/>
    </figure>
    <p>
      We sometimes call <m>g</m> the
      <q>inner function</q>
      and <m>f</m> the
      <q>outer function</q>. It is important to note that the inner function is actually the first function that gets applied to a given input,
      and then outer function is applied to the output of the inner function.
      In addition, in order for a composite function to make sense,
      we need to ensure that the range of the inner function lies within the domain of the outer function so that the resulting composite function is defined at every possible input.
    </p>
    <p>
      In the following examples,
      we consider compositions of functions given by tables,
      then by graphs, and finally by formulas.
    </p>
    <example xml:id="ex_compositionbytables">
      <statement>
        <p>
          Suppose that <m>f</m> and <m>g</m> are given by the table
        </p>
        <p>
          <image width="28%" source="APCTable1-6-3.png"/>
        </p>
        <p>
          This means, for example, that <m>f(0)=6</m>, <m>f(1)=4</m>,
          <m>f(2) = 3</m>, etc., and that <m>g(0)=1, g(1)=3, g(2)=0</m>, etc.
        </p>
        <p>
          We can calculate <m>(f\circ g)(2) = f(g(2))</m>.
          Since <m>g(2) = 0</m> and <m>f(0) = 6</m>,
          <m>f(g(2)) = f(0) = 6</m>.
        </p>
        <p>
          We can also calculate <m>(g\circ f)(2) = g(f(2))</m>.
          Since <m>f(2) = 3</m> and <m>g(3)=4</m>, <m>g(f(2)) = 4</m>.
        </p>
      </statement>
    </example>
    <exercise>
      <statement>
        <p>
          For <m>f</m> and <m>g</m> as in Example <xref ref="ex_compositionbytables" autoname="yes"/>,
          compute each of the following quantities or explain why they are not defined.
          <ol marker="labelalph">
            <li>
              <p>
                <m>(g\circ f)(3)</m>
              </p>
            </li>
            <li>
              <p>
                <m>g(f(0))</m>
              </p>
            </li>
            <li>
              <p>
                For what value(s) of <m>x</m> is <m>f(g(x))=4</m>?
              </p>
            </li>
          </ol>
        </p>
      </statement>
    </exercise>
    <example xml:id="ex_compositionbygraphs">
      <statement>
        <p>
          If <m>p</m> and <m>q</m> are given by the graphs
        </p>
        <p>
          <image width="50%" source="APCFigure1-6-4.png"/>
        </p>
        <p>
          then <m>(p\circ q)(0) = p(q(0))</m>.
          Since <m>q(0) = 2</m> and <m>p(2) = 2</m>,
          <m>p(q(0)) = p(2) = 2</m>.
        </p>
      </statement>
    </example>
    <exercise>
      <statement>
        <p>
          For <m>p</m> and <m>q</m> as in Example <xref ref="ex_compositionbygraphs" autoname="yes"/>,
          compute each of the following quantities or explain why they are not defined.
          <ol marker="labelalph">
            <li>
              <p>
                <m>(q\circ p)(0)</m>
              </p>
            </li>
            <li>
              <p>
                <m>(p\circ p)(-1.5)</m>
              </p>
            </li>
            <li>
              <p>
                <m>(q\circ p)(2)</m>
              </p>
            </li>
          </ol>
        </p>
      </statement>
    </exercise>
    <example xml:id="ex_compositionbyformulas">
      <statement>
        <p>
          Suppose that
          <me>
            f(x) = x^2-1
          </me>
          and that
          <me>
            g(x) = 3x-\frac{4}{x}
          </me>
        </p>
        <p>
          The composition <m>f\circ g</m> means that we use <m>g(x)</m> as the inputs for the function <m>f</m>.
          Think of <m>f</m> as the process that squares its input,
          then subtracts 1:
          <me>
            f(?) = (?)^2-1
          </me>
        </p>
        <p>
          If the input is <m>g(x) = 3x-\frac{4}{x}</m>, we can simplify:
          <me>
            \begin{aligned}(f\circ g)(x) \amp = f(g(x))\\ \amp = (g(x))^2-1\\ \amp = \left(3x-\frac{4}{x}\right)^2-1 \end{aligned}
          </me>
        </p>
        <p>
          We could simplify this further if we wanted to,
          thought it isn't really necessary:
          <me>
            \begin{aligned}(f\circ g)(x) \amp = \left(3x-\frac{4}{x}\right)^2-1\\ \amp = \left(9x^2-24+\frac{16}{x^2}\right)-1\\ \amp = 9x^2+\frac{16}{x^2}-25 \end{aligned}
          </me>
        </p>
        <p>
          We could also compose the other direction.
          The composition <m>g\circ f</m> means that we use <m>f(x)</m> as the inputs for the function <m>g</m>.
          Think of <m>g</m> as the function that multiplies 3 times its input,
          divides 4 by its input, then subtracts the latter from the former:
          <me>
            g(?) = 3(?)-\frac{4}{?}
          </me>
        </p>
        <p>
          If the input is <m>f(x) = x^2-1</m>,
          <me>
            \begin{aligned}(g\circ f)(x) \amp = g(f(x))\\ \amp = 3(f(x))-\frac{4}{f(x)}\\ \amp = 3(x^2-1)-\frac{4}{x^2-1} \end{aligned}
          </me>
        </p>
        <p>
          We could simplify a littler further if we wanted to by distributing the 3, but anything farther would be a waste of time (like writing it as a single fraction over a common denominator):
          <me>
            \begin{aligned}(g\circ f)(x) \amp = 3(x^2-1)-\frac{4}{x^2-1}\\ \amp = 3x^2-3-\frac{4}{x^2-1} \end{aligned}
          </me>
        </p>
      </statement>
    </example>
    <exercise xml:id="ex_compositionbyformulas2">
      <statement>
        <p>
          Let <m>p(x) = \frac{1}{x+4}</m> and <m>q(x) = x^2-4</m>.
          <ol marker="labelalph">
            <li>
              <p>
                Find and simplify
                (as much as is reasonable)
                a formula for <m>p\circ q</m>.
              </p>
            </li>
            <li>
              <p>
                Find and simplify
                (as much as is reasonable)
                a formula for <m>q\circ p</m>.
              </p>
            </li>
          </ol>
        </p>
      </statement>
    </exercise>
    <example>
      <statement>
        <p>
          Suppose that <m>h(x) = \sqrt{2x^2+5}</m>.
          Determine formulas for two related functions,
          <m>f(x)</m> and <m>g(x)</m>, so that <m>h(x) = f(g(x))</m>.
        </p>
      </statement>
      <solution>
        <p>
          One possibility is that <m>f(x) = \sqrt{x}</m> and <m>g(x) = 2x^2+5</m>.
        </p>
        <p>
          Another possibility is that
          <m>f(x) = \sqrt{2x+5}</m> and <m>g(x) = x^2</m>.
        </p>
        <p>
          Do you see any additional possibilities?
        </p>
      </solution>
    </example>
    <p>
      \fbox{ <em>Important!</em> Function composition is
      <em>not at all</em> like multiplication.
      As we have seen in Example <xref ref="ex_compositionbyformulas" autoname="yes"/> and Exercise <xref ref="ex_compositionbyformulas2" autoname="yes"/>,
      it is not necessarily true that
      <m>f\circ g = g\circ f</m> or that <m>p\circ q = q\circ p</m>.
      In fact, that is usually not true at all. }
    </p>
  </subsection>
  <subsection>
    <title>Domain of Compositions</title>
    <p>
      Suppose we have two functions,
      <m>y=f(x)</m> and <m>x=g(t)</m>.
      The domain of <m>f\circ g</m> is the set of all <m>t</m> in the domain of <m>g</m> such that <m>x=g(t)</m> is in the domain of <m>f</m>.
      In other words,
      <m>(f\circ g)(t)</m> is defined whenever both <m>g(t)</m> and <m>f(g(t))</m> are defined.
    </p>
    <example>
      <statement>
        <p>
          For <m>y=f(x) = \frac{1}{x}</m> and <m>x=g(t) = \sqrt{t+1}</m>,
          we find the domain of <m>f\circ g</m>.
        </p>
        <p>
          For a value <m>t</m> to be in the domain of <m>f\circ g</m>,
          it must first be in the domain <m>[-1,\infty)</m> of <m>g</m>.
          Then the value of <m>g(t) = \sqrt{t+1}</m> must be in the domain of <m>f</m>,
          so we must have <m>\sqrt{t+1}\neq 0</m>,
          or in other words, <m>t\neq 1</m>.
          Therefore the domain of <m>f\circ g</m> is <m>(-1,\infty)</m>.
        </p>
        <p>
          For values of <m>t</m> in this domain, we have
          <me>
            (f\circ g)(t) = f(g(t)) = f(\sqrt{t+1}) = \frac{1}{\sqrt{t+1}}
          </me>.
          Notice that this equation is consistent with our calculation of the domain.
        </p>
      </statement>
    </example>
    <exercise>
      <statement>
        <p>
          For <m>y=g(x) =\sqrt{x+1}</m> and <m>x=f(t) = \dfrac{1}{t}</m>,
          find the domain of <m>g\circ f</m>.
        </p>
      </statement>
    </exercise>
    <example>
      <statement>
        <p>
          Recall the functions <m>f(x) = x^2-1</m> and
          <m>g(x) = 3x-\frac{4}{x}</m> from Example <xref ref="ex_compositionbyformulas" autoname="yes"/>.
          Let's find the domains of <m>f\circ g</m> and <m>g\circ f</m>.
        </p>
        <p>
          The domain of <m>g(x)</m> is <m>x\neq 0</m>.
          The domain of <m>f(x)</m> is all real numbers,
          so there is no need to limit the outputs of <m>g</m>.
          Hence the domain is <m>(-\infty,0)\cup (0,\infty)</m>.
          We found a simplified formula of
          <me>
            (f\circ g)(x) = 9x^2+\frac{16}{x^2}-25
          </me>,
          which agrees with our previous analysis.
        </p>
        <p>
          In the other direction,
          the domain of <m>f(x) = x^2-1</m> has no restrictions,
          but when we plug <m>f(x)</m> into <m>g(x) = 3x-\frac{4}{x}</m>,
          we notice that this requires the input to be nonzero because of the <m>x</m> in the denominator,
          hence we must have <m>f(x) = x^2-1\neq 0</m> in order for <m>g(f(x))</m> to be defined.
          Thus the domain for <m>g\circ f</m> should be <m>x\neq \pm1</m>.
          Indeed, we found a simplified formula of
          <me>
            (g\circ f)(x) = 3x^2-3-\frac{4}{x^2-1}
          </me>
        </p>
        <p>
          Since <m>x^2-1</m> is in the denominator,
          we cannot have <m>x=1</m> or <m>x=-1</m>.
          Thus the domain is indeed <m>(-\infty,-1)\cup(-1,1)\cup(1,\infty)</m>.
        </p>
      </statement>
    </example>
    <example>
      <title>A Cautionary Example</title>
      <statement>
        <p>
          Let's consider the functions
          <m>f(x) =g(x) = \frac{1}{x}</m> and look at the domain of <m>f\circ g</m>.
          If we view <m>g(x)</m> as the first function applied to <m>x</m>,
          we know that we must have <m>x\neq 0</m>.
        </p>
        <p>
          However, if we first simplify the formula for the composition:
          <me>
            \begin{aligned}(f\circ g)(x) \amp = f(g(x))\\ \amp = \frac{1}{g(x)}\\ \amp =\frac{1}{1/x}\\ \amp = x \end{aligned}
          </me>
          we might think that the domain is all real numbers, which would be incorrect!
        </p>
      </statement>
    </example>
    <p>
      \fbox{ <em>Remember!</em> The domain of
      <m>(f\circ g)(x)</m> is the values of <m>x</m> in the domain of <m>g</m> so that the output of <m>g(x)</m> is <em>also</em>
      in the domain of <m>f</m>. }
    </p>
  </subsection>
  <subsection>
    <title>Function Composition and Average Rate of Change</title>
    <p>
      In this section,
      we see how the idea of composition can be used in concert with the formula for average rate of change.
      You have already seen a few WeBWorK problems that involve doing this!
      Hopefully this section clears up any lingering confusion.
    </p>
    <p>
      Recall that the average rate of change of a function <m>f</m> on the interval <m>[a,b]</m> is given by
      <me>
        AV_{[a,b]} = \frac{f(b)-f(a)}{b-a}
      </me>.
      In the figure below, we see the familiar representation of
      <m>AV_{[a,b]}</m> as the slope of the line joining the points <m>(a,f(a))</m> and
      <m>(b,f(b))</m> on the graph of <m>f</m>.
      In the study of calculus,
      we progress from the <em>average rate of change on an interval</em>
      to the <em>instantaneous rate of change</em>
      of a function at a single value
      (what we might want to call the "slope" of a nonlinear curve).
      The core idea that allows us to move from an <em>average</em>
      rate to an <em>instantaneous</em>
      one is letting the interval <m>[a,b]</m> shrink in size.
    </p>
    <p>
      To think about the interval <m>[a,b]</m> shrinking while <m>a</m> stays fixed,
      we often change our perspective and think of <m>b</m> as <m>a+h</m>,
      where <m>h</m> measures the horizontal difference from <m>b</m> to <m>a</m>.
      See <xref ref="fig_abtoaplush" autoname="yes"/> below.
    </p>
    <figure xml:id="fig_abtoaplush">
      <caption>Think of the interval <m>[a,b]</m> as the interval <m>[a,a+h]</m>.</caption>
      <image width="70%" source="APCFigure1-6-7-8.png"/>
    </figure>
    <p>
      This allows us to eventually think about <m>h</m> getting closer and closer to <m>0</m>,
      and in that context we consider the equivalent expression
      <me>
        AV_{[a,a+h]}  = \frac{f(a+h)-f(a)}{(a+h)-a} =\frac{f(a+h)-f(a)}{h}
      </me>
      for the average rate of change of <m>f</m> on <m>[a,a+h]</m>.
    </p>
    <p>
      In this most recent expression for <m>AV_{[a,a+h]}</m>,
      we see the important role that the composite function "<m>f(a+h)</m>" plays.
      In particular, to understand the expression for
      <m>AV_{[a,a+h]}</m> we need to evaluate <m>f</m> at the quantity <m>(a+h)</m>.
    </p>
    <example xml:id="ex_APC1-6-9">
      <statement>
        <p>
          Suppose that <m>f(x) = x^2+1</m>.
          Determine the simplest possible expression you can find for <m>AV_{[3,3+h]}</m>,
          the average rate of change of <m>f</m> on the interval <m>[3,3+h]</m>.
        </p>
      </statement>
      <solution>
        <p>
          By definition, we know that
          <me>
            AV_{[3,3+h]} = \frac{f(3+h)-f(3)}{h}
          </me>
        </p>
        <p>
          Using the formula for <m>f</m>,
          we have <m>f(3+h) = (3+h)^2+1</m> and <m>f(3) = 3^2+1</m>, so that
          <me>
            AV_{[3,3+h]} = \frac{((3+h)^2+1)-(3^2+1)}{h}
          </me>
        </p>
        <p>
          Expanding the numerator and combining like terms, it follows that
          <me>
            \begin{aligned}AV_{[3,3+h]} \amp = \frac{9+6h+h^2+1-10}{h}\\ \amp = \frac{6h+h^2}{h}\\ \amp =\frac{h(6+h)}{h}\\ \amp = 6+h. \end{aligned}
          </me>
        </p>
        <p>
          Hence <m>AV_{[3,3+h]} = 6+h</m>,
          which is the average rate of change of
          <m>f(x) = x^2+1</m> on the interval <m>[3,3+h]</m>.
        </p>
      </solution>
    </example>
    <exercise>
      <statement>
        <ol marker="labelalphitemsep10pt">
          <li>
            <p>
              Rewrite each interval <m>[3,4]</m>, <m>[3,3.5]</m>,
              <m>[3,3.1]</m> in the form <m>[3,3+h]</m> for some value of <m>h</m>.
              What is <m>h</m> for each interval.
            </p>
          </li>
          <li>
            <p>
              Confirm the formula <m>AV_{[3,3+h]}=6+h</m> from <xref ref="ex_APC1-6-9">Example</xref>
              by calculating the average rate of change of
              <m>f(x) = x^2+1</m> on <m>[3,4]</m>, <m>[3,3.5]</m>,
              and <m>[3,3.1]</m> using the original formula
              <m>AV_{[a,b]} = \frac{f(b)-f(a)}{b-a}</m> and comparing it to the value of <m>6+h</m>.
            </p>
          </li>
          <li>
            <p>
              What would you estimate the "instantaneous" rate of change of <m>f(x) = x^2+1</m> at <m>x=3</m> to be,
              based on this calculation?
              Remember that the instantaneous rate of change is what we get as we let the interval <m>[3,3+h]</m> get smaller and smaller.
            </p>
          </li>
        </ol>
      </statement>
    </exercise>
  </subsection>
  <subsection>
    <title>Summary</title>
    <p>
      The following terms were introduced in this section:
    </p>
    composition of functions, instantaneous rate of change
    <p>
      <em>Key ideas:</em> The composition
      <m>(f\circ g)(x) = f(g(x))</m> means to use <m>g(x)</m> as the input of the function <m>f</m>.
      The domain of <m>f\circ g</m> is a subset of the domain of <m>g</m> so that <m>g(x)</m> is in the domain of <m>f</m>.
    </p>
    <p>
      <em>Other ideas introduced:</em>
      Composition of functions plays an important role in defining the instantaneous rate of change of a function,
      which is a central idea in calculus.
    </p>
    <p>
      \fbox{\fbox{ End of Section 1.9}}
    </p>
    <p>
      \rule{1.1\textwidth}{2pt}
    </p>
  </subsection>
</section>